theorems/experiments/denote_IR_3.lean
@@ -1,0 +1,146 @@
+import theorems.iN
+
+import Lean
+import Qq
+open Lean Elab Meta
+open Qq
+
+inductive IR : Nat → Type where
+  | var (id : Nat) : IR idx
+  | const (val : Nat) : IR idx
+  | const_poison : IR idx
+
+  | add (lhs rhs : IR idx) : IR idx
+  | addNsw (lhs rhs : IR idx) : IR idx
+deriving BEq, Repr
+
+deriving instance BEq for iN
+
+structure PackediN where
+  {n : Nat}
+  x : iN n
+deriving BEq
+
+def PackediN.truncate (pack : PackediN) (n : Nat) : iN n :=
+  match pack.x with
+  | poison => poison
+  | bitvec a => a.truncate n
+
+abbrev Assignment := Lean.RArray PackediN
+abbrev WidthAssignment := Lean.RArray Nat
+
+namespace IR
+
+def eval (ξ : WidthAssignment) (σ : Assignment) : IR idx → iN (ξ.get idx)
+  | var id =>
+    let pack := σ.get id
+    /- h is always true, this if is for totality -/
+    if h : pack.n = (ξ.get idx) then
+      h ▸ pack.x
+    else
+      pack.truncate (ξ.get idx)
+
+  | const val => bitvec val
+  | const_poison => poison
+
+  | add lhs rhs => iN.add (eval ξ σ lhs) (eval ξ σ rhs)
+  | addNsw lhs rhs => iN.addNsw (eval ξ σ lhs) (eval ξ σ rhs)
+
+  /- | add lhs rhs => iN.add (eval σ lhs) (eval σ rhs)
+  | addNsw lhs rhs => iN.addNsw (eval σ lhs) (eval σ rhs)
+  | addNuw lhs rhs => iN.addNuw (eval σ lhs) (eval σ rhs)
+  | addNw lhs rhs => iN.addNw (eval σ lhs) (eval σ rhs) -/
+
+end IR
+
+theorem add_zero {n} (x : iN n) : x + (bitvec 0) ~> x := by
+  poison_unroll x => a
+  simp [simp_iN]
+
+/--
+For the implementation to optimise, it needs to know whether or not the width assignment respect the `valid` prop.
+--/
+structure Rule where
+  valid : WidthAssignment → Bool
+
+  impl : (ξ : WidthAssignment) → valid ξ → {idx : Nat} → IR idx → IR idx
+
+  wf : ∀ (ξ : WidthAssignment) (h : valid ξ) (σ : Assignment) {idx : Nat} (lhs : IR idx),
+    let rhs := impl ξ h lhs
+    (IR.eval ξ σ lhs) ~> (IR.eval ξ σ rhs)
+
+def add_zero' : Rule :=
+  { valid := fun ξ => true
+  , impl := fun ξ _ _ ir => match ir with
+      | IR.add lhs (IR.const 0) => lhs
+      | _ => ir
+  , wf := by
+      intros ξ _ σ _ lhs
+
+      split <;> try rfl
+      apply add_zero
+  }
+
+def applyRewrite {idx} (ir : IR idx) (r : Rule) (ξ : WidthAssignment) (ξvalid : r.valid ξ) : IR idx :=
+  r.impl ξ ξvalid ir
+
+theorem applyRewriteCorrect (ir : IR idx) (r : Rule)
+  (σ : Assignment) (ξ : WidthAssignment) (ξvalid : r.valid ξ)
+  : (IR.eval ξ σ ir) ~> (IR.eval ξ σ (applyRewrite ir r ξ ξvalid)) := r.wf ξ ξvalid σ ir
+
+def A : IR 0 := IR.add (IR.var 0) (IR.const 0)
+def B {n : Nat} : IR 0 := applyRewrite A add_zero' (Lean.RArray.leaf n) (by trivial)
+
+def Aeval {n} : iN n → iN n :=
+  fun x => IR.eval (Lean.RArray.leaf n) (Lean.RArray.leaf ⟨x⟩) A
+
+def Beval {n} : iN n → iN n :=
+  fun x => IR.eval (Lean.RArray.leaf n) (Lean.RArray.leaf ⟨x⟩) (@B n)
+
+theorem Aeval_rewrite_Beval {n} (x : iN n) :
+  Aeval x ~> Beval x :=
+  applyRewriteCorrect A add_zero' (Lean.RArray.leaf ⟨x⟩) (Lean.RArray.leaf n) (by trivial)
+
+#eval @Aeval 32 (bitvec 1)
+
+theorem addNsw_refine_add {n} (x y : iN n) : x +nsw y ~> x + y := by
+  poison_unroll x y => a b
+
+  by_cases h : a.saddOverflow b
+  . rw [addNsw_saddOverflow_bitvec h]
+    exact Rewrite.poison_rewrite (bitvec a + bitvec b)
+  . rw [addNsw_not_saddOverflow_bitvec_eq_add h]
+    simp [simp_iN]
+
+def addNsw_refine_add' : Rule :=
+  { valid := fun ξ => true
+  , impl := fun ξ _ _ ir => match ir with
+      | IR.addNsw lhs rhs => IR.add lhs rhs
+      | _ => ir
+
+  , wf := by
+      intros ξ _ σ _ lhs
+
+      split <;> try rfl
+      apply addNsw_refine_add
+  }
+
+def Cσ (x y : iN n) : Assignment :=
+  .ofArray #[⟨x⟩, ⟨y⟩] (by simp)
+
+/- program C is optimised into program D -/
+def C : IR 0 := IR.addNsw (IR.var 0) (IR.var 1)
+def D {n : Nat} : IR 0 := applyRewrite C addNsw_refine_add' (.leaf n) (by trivial)
+
+/- Ceval is the actual denoted semantics behind C, same for Deval -/
+def Ceval {n} (x y : iN n) : iN n := IR.eval (.leaf n) (Cσ x y) C
+def Deval {n} (x y : iN n) : iN n := IR.eval (.leaf n) (Cσ x y) (@D n)
+
+/- correctness proof -/
+theorem Ceval_rewrite_Deval {n} (x y : iN n) :
+  Ceval x y ~> Deval x y :=
+  applyRewriteCorrect C addNsw_refine_add' (Cσ x y) (.leaf n) (by trivial)
+
+/- but, behaviour is not equal! the behaviour of C is "refined" into D -/
+#eval @Ceval 32 (bitvec 2147483647) (bitvec 1) /- iN.poison -/
+#eval @Deval 32 (bitvec 2147483647) (bitvec 1) /- iN.bitvec 0x80000000#32 -/
